first attempt at using LockR

templates/lock.v
@@ -13,7 +13,7 @@ Section Lock_module.
   (** Assumed functions to retrieve lock bit from a node *)
   Parameter lockLoc : Node → loc.
   Parameter getLockLoc : val.
-
+  
   Parameter getLockLoc_spec : ∀ (n: Node),
     ⊢ ({{{ True }}}
         getLockLoc #n
@@ -35,25 +35,31 @@ Section Lock_module.
     
   (** Lock module proofs *)
 
-  Lemma lockNode_spec (n: Node):
-    ⊢ <<< ∀ (b: bool), (lockLoc n) ↦ #b >>>
+  Definition lockR (b: bool) (n: Node) (R: iProp Σ) : iProp Σ :=
+    ((lockLoc n) ↦ #b ∗ (if b then True else R))%I.
+  
+  Lemma lockNode_spec (n: Node) (R: iProp Σ):
+    ⊢ <<< ∀ b, lockR b n R >>>
       lockNode #n    @ ⊤
-    <<< (lockLoc n) ↦ #true ∗ ⌜b = false⌝ , RET #() >>>.
+    <<< lockR true n R ∗ R, RET #() >>>.
   Proof.
     iIntros (Φ) "AU". iLöb as "IH".
     wp_lam. wp_bind(getLockLoc _)%E.
     wp_apply getLockLoc_spec; first done.
     iIntros (l) "#Hl". wp_let. wp_bind (CmpXchg _ _ _)%E.
     iMod "AU" as (b) "[Hb HAU]". iDestruct "Hl" as %Hl.
+    unfold lockR.
     iEval (rewrite Hl) in "Hb". destruct b.
-    - wp_cmpxchg_fail. iDestruct "HAU" as "[HAU _]".
+    - iDestruct "Hb" as "[Hb Htrue]".
+      wp_cmpxchg_fail. iDestruct "HAU" as "[HAU _]".
       iEval (rewrite Hl) in "HAU".
-      iMod ("HAU" with "Hb") as "H".
+      iMod ("HAU" with "[$Hb $Htrue]") as "H".
       iModIntro. wp_pures. iApply "IH".
       iEval (rewrite <-Hl) in "H". done.
-    - wp_cmpxchg_suc. iDestruct "HAU" as "[_ HAU]".
+    - iDestruct "Hb" as "[Hb HR]".
+      wp_cmpxchg_suc. iDestruct "HAU" as "[_ HAU]".
       iEval (rewrite Hl) in "HAU".
-      iMod ("HAU" with "[Hb]") as "HΦ". iFrame; done.
+      iMod ("HAU" with "[Hb HR]") as "HΦ". iFrame; done.
       iModIntro. wp_pures. done.
   Qed.
 
