templates/single_node.v
@@ -163,8 +163,7 @@ Section One_Node_Template.
   Definition CSS γ r (C: gset K) : iProp :=
     ∃ (b: bool),
       γ ⤇½ C
-      ∗ lockLoc r ↦ #b
-      ∗ (if b then True else nodePred γ r C).
+      ∗ lockR b r (nodePred γ r C).
 
   (** High-level lock specs **)
 
@@ -173,20 +172,27 @@ Section One_Node_Template.
          lockNode #r @ ⊤
        <<< CSS γ r C ∗ nodePred γ r C, RET #() >>>.
   Proof.
-    iIntros (Φ) "AU".
-    awp_apply (lockNode_spec r).
-    iApply (aacc_aupd_commit with "AU"); first done.
-    iIntros (C) "Hcss". iDestruct "Hcss" as (b) "(HC & Hlock & Hb)".
-    iAaccIntro with "Hlock".
-    { iIntros "Hlockn". iModIntro. iSplitL.
-      iFrame. iExists b. iFrame.
-      eauto with iFrame.
-    }
-    iIntros "(Hlockn & %)". iModIntro.
-    subst b. iSplitL.
-    iFrame. iExists true. iFrame.
-    eauto with iFrame.
-  Qed.
+    iIntros (Φ) "AU". iLöb as "IH".
+    wp_lam. wp_bind(getLockLoc _)%E.
+    wp_apply getLockLoc_spec; first done.
+    iIntros (l) "#Hl". wp_let. 
+    wp_bind (CmpXchg _ _ _)%E.
+    iMod "AU" as (C) "[HC HAU]".
+    iDestruct "HC" as (b) "(Hfrac & HlockR)". 
+    iDestruct "HlockR" as "(HlockLoc & Hlockif)". iDestruct "Hl" as %Hl.
+    iEval (rewrite Hl) in "HlockLoc". destruct b.
+    - iDestruct "HlockLoc" as "[HlockLoc Htrue]".
+      wp_cmpxchg_fail. iDestruct "HAU" as "[HAU _]".
+      iMod ("HAU" with "[HlockLoc Htrue Hfrac]") as "H".
+      iExists true. unfold lockR. iFrame.
+      iEval (rewrite Hl). iFrame.   
+      iModIntro. wp_pures. iApply "IH". done.
+    - wp_cmpxchg_suc. iDestruct "HAU" as "[_ HAU]".
+      iMod ("HAU" with "[HlockLoc Hlockif Hfrac]") as "HΦ".
+      iFrame. iExists true. unfold lockR. 
+      iEval (rewrite Hl). iFrame.
+      iModIntro. wp_pures. done.
+Qed.
 
   (** Proof of CSSOp *)
 
